SmallStep.v
@@ -12,45 +12,84 @@ Require Import LLIR.Dom.
 Require Import LLIR.Eval.
 Require Import LLIR.SSA.
 Require Import LLIR.Block.
+Require Import LLIR.Typing.
 
 Import ListNotations.
-
-
 
 Inductive event: Type.
 
 Definition trace := list event.
 
-Definition stk_state := list frame.
+Definition stack := (positive, PTrie.t frame).
 
-Axiom mem_state: Type.
-
-Inductive state: Type :=
-  | State:
-      forall
-        (stk: stk_state)
-        (mem: mem_state)
-        (pc: node),
-        state
+Inductive Heap: Type :=
   .
 
-Definition get_inst (p: prog) (stk: stk_state) (pc: node): option inst :=
+(*
+Inductive state: Type :=
+  | State:
+    forall
+      (stk: stack)
+      (mem: Heap),
+      state
+  | Exit:
+    forall
+      (stk: PTrie.t frame)
+      (mem: Heap),
+      state
+  .
+
+Inductive Final: state -> Prop :=
+  | final_exit:
+    forall (stk: PTrie.t frame) (mem: Heap),
+      Final (Exit stk mem)
+  .
+
+Inductive Executing: prog -> Stack -> inst -> Prop :=
+  | executing:
+    forall (p: prog) (stk
+    
+
+
+Definition get_inst (p: prog) (stk: Stack): option inst :=
   match stk with
-  | f :: _ =>
-    match p ! (f.(fr_func)) with
-    | Some func => func.(fn_insts) ! pc
+  | stack fr _ _ =>
+    match p ! (fr.(fr_func)) with
+    | Some func => func.(fn_insts) ! (fr.(fr_pc))
     | None => None
     end
-  | _ => None
   end.
 
-Axiom get_vreg: stk_state -> reg -> option value.
+Definition get_vreg (stk: stk_state) (r: reg): value :=
+  match stk with
+  | (fr, _) => get_vreg fr r
+  end.
 
-Axiom set_vreg: stk_state -> reg -> value -> option stk_state.
+Definition set_pc (stk: stk_state) (pc: node): stk_state :=
+  match stk with
+  | (fr, frs) => (set_pc fr pc, frs)
+  end.
 
-Axiom is_true: value -> Prop.
+Definition set_vreg (stk: stk_state) (r: reg) (v: value): stk_state :=
+  match stk with
+  | (fr, frs) => (set_vreg fr r v, frs)
+  end.
 
-Axiom is_false: value -> Prop.
+Definition set_vreg_pc (stk: stk_state) (r: reg) (v: value) (pc: node): stk_state :=
+  match stk with
+  | (fr, frs) => (set_vreg_pc fr r v pc, frs)
+  end.
+
+Lemma value_tf_dec: forall (v: value), IsTrue v \/ IsFalse v.
+Proof.
+  intros v; destruct v.
+  - destruct (INT8.eq_dec  v INT8.zero);  [right; subst|left]; constructor; auto.
+  - destruct (INT16.eq_dec v INT16.zero); [right; subst|left]; constructor; auto.
+  - destruct (INT32.eq_dec v INT32.zero); [right; subst|left]; constructor; auto.
+  - destruct (INT64.eq_dec v INT64.zero); [right; subst|left]; constructor; auto.
+  - left; constructor.
+  - right; constructor.
+Qed.
 
 Axiom eval_unop: ty -> unop -> value -> option value.
 
@@ -62,74 +101,79 @@ Inductive step (p: prog): state -> trace -> state -> Prop :=
       (stk: stk_state) (mem: mem_state) (tr: trace)
       (pc: node)
       (target: node),
-      get_inst p stk pc = Some (LLJmp target) ->
+      get_inst p stk = Some (LLJmp target) ->
       step
         p
-        (State stk mem pc)
+        (State stk mem)
         tr
-        (State stk mem target)
+        (State (set_pc stk target) mem)
   | eval_jcc_true:
     forall
       (stk: stk_state) (mem: mem_state) (tr: trace)
-      (pc: node)
-      (cond: reg) (brancht: node) (branchf: node)
-      (v: value),
-      get_inst p stk pc = Some (LLJcc cond brancht branchf) ->
-      get_vreg stk cond = Some v ->
-      is_true v ->
+      (cond: node) (pc: node)
+      (brancht: node) (branchf: node),
+      get_inst p stk = Some (LLJcc cond brancht branchf) ->
+      IsTrue (get_vreg stk cond) ->
       step
         p
-        (State stk mem pc)
+        (State stk mem)
         tr
-        (State stk mem brancht)
+        (State (set_pc stk brancht) mem)
   | eval_jcc_false:
     forall
       (stk: stk_state) (mem: mem_state) (tr: trace)
-      (pc: node)
-      (cond: reg) (brancht: node) (branchf: node)
-      (v: value),
-      get_inst p stk pc = Some (LLJcc cond brancht branchf) ->
-      get_vreg stk cond = Some v ->
-      is_false v ->
+      (cond: node) (pc: node)
+      (brancht: node) (branchf: node),
+      get_inst p stk = Some (LLJcc cond brancht branchf) ->
+      IsFalse (get_vreg stk cond) ->
       step
         p
-        (State stk mem pc)
+        (State stk mem)
         tr
-        (State stk mem brancht)
+        (State (set_pc stk brancht) mem)
   | eval_unary:
     forall
       (stk: stk_state) (mem: mem_state) (tr: trace)
       (pc: node)
       (ty: ty) (op: unop) (arg: reg) (dst: reg) (next: node)
-      (arg_value: value) (dst_value: value)
-      (stk': stk_state),
-      get_inst p stk pc = Some (LLUnop (ty, dst) next op arg) ->
-      get_vreg stk arg = Some arg_value ->
-      eval_unop ty op arg_value = Some dst_value ->
-      set_vreg stk dst dst_value = Some stk' ->
+      (dst_value: value),
+      get_inst p stk = Some (LLUnop (ty, dst) next op arg) ->
+      eval_unop ty op (get_vreg stk arg) = Some dst_value ->
       step
         p
-        (State stk mem pc)
+        (State stk mem)
         tr
-        (State stk' mem next)
+        (State (set_vreg_pc stk dst dst_value next) mem)
   | eval_binary:
     forall
       (stk: stk_state) (mem: mem_state) (tr: trace)
       (pc: node)
       (ty: ty) (op: binop) (lhs: reg) (rhs: reg) (dst: reg) (next: node)
-      (lhs_value: value) (rhs_value: value) (dst_value: value)
-      (stk': stk_state),
-      get_inst p stk pc = Some (LLBinop (ty, dst) next op lhs rhs) ->
-      get_vreg stk lhs = Some lhs_value ->
-      get_vreg stk rhs = Some rhs_value ->
-      eval_binop ty op lhs_value rhs_value = Some dst_value ->
-      set_vreg stk dst dst_value = Some stk' ->
+      (dst_value: value),
+      get_inst p stk = Some (LLBinop (ty, dst) next op lhs rhs) ->
+      eval_binop ty op (get_vreg stk lhs) (get_vreg stk rhs) = Some dst_value ->
       step
         p
-        (State stk mem pc)
+        (State stk mem)
         tr
-        (State stk' mem next)
+        (State (set_vreg_pc stk dst dst_value next) mem)
   .
+
+Theorem well_typed_progress:
+  forall (p: prog) (st: state),
+    well_typed_prog p ->
+    ~Final st ->
+    exists (tr: trace) (st': state),
+      step p st tr st'.
+Proof.
+  intros p st Hty Hfinal.
+  destruct st.
+  {
+    clear Hfinal.
+    destruct stk; destruct f.
+  }
+  { assert (Final (Exit stk mem)). constructor. contradiction. }
+Qed.
 
 Inductive star (p: prog): state -> trace -> state -> Prop :=
   | star_refl:
@@ -163,13 +207,13 @@ Inductive ExecutionAt (p: prog): stk_state -> mem_state -> func -> node -> Prop 
     forall
       (fr_data: PTrie.t atom) (fr_regs: PTrie.t value) (fr_args: PTrie.t value)
       (fr_func: name) (fr_pc: node) (fr_retaddr: node)
-      (frs: list frame) (mem: mem_state) (f: func)
+      (frs: PTrie.t frame) (mem: mem_state) (f: func)
       (FUNC: Some f = p ! fr_func)
       (INST: None <> f.(fn_insts) ! fr_pc)
       (r: reg),
       ExecutionAt
         p
-        (mkframe fr_data fr_regs fr_args fr_func fr_pc fr_retaddr :: frs)
+        (mkframe fr_data fr_regs fr_args fr_func fr_pc fr_retaddr, frs)
         mem
         f
         fr_pc
@@ -180,6 +224,7 @@ Section FUNCTION.
   Hypothesis f_is_valid: is_valid f.
 
   Definition has_header := fn_blocks_are_valid f f_is_valid.
+
   (*
   Theorem exec_bb:
     forall (h: node) (n: node),
@@ -220,3 +265,4 @@ Section FUNCTION.
   *)
 
 End FUNCTION.
+*)
