Values.v
@@ -20,15 +20,79 @@ Inductive bit : Type :=
   .
 
 Module Type VALUE.
-  Parameter t : Type.
+  Parameter t: Type.
+
+  Parameter is_zero: t -> bool.
+
+  Parameter zero: t.
+
+  Parameter eq_dec: forall (x: t) (y: t), {x = y} + {x <> y}.
+
+  Parameter zero_is_zero: is_zero zero = true.
+
+  Parameter non_zero_is_not_zero: forall (x: t), x <> zero -> is_zero x = false.
 End VALUE.
 
 Module DOUBLE (BASE : VALUE).
   Definition t := (BASE.t * BASE.t)%type.
+
+  Definition is_zero v :=
+    match v with
+    | (lo, hi) => BASE.is_zero lo && BASE.is_zero hi
+    end.
+
+  Definition zero: t := (BASE.zero, BASE.zero).
+
+  Lemma eq_dec: forall (x: t) (y: t), {x = y} + {x <> y}.
+  Proof.
+    intros x y.
+    destruct x; destruct y.
+    destruct (BASE.eq_dec t0 t2); destruct (BASE.eq_dec t1 t3); subst; auto;
+    right; intros contra; inversion contra; contradiction.
+  Qed.
+
+  Lemma zero_is_zero: is_zero zero = true.
+  Proof.
+    simpl; rewrite BASE.zero_is_zero; auto.
+  Qed.
+
+  Lemma non_zero_is_not_zero: forall (x: t), x <> zero -> is_zero x = false.
+  Proof.
+    intros x Hnz.
+    destruct x as [lo hi].
+    destruct (BASE.eq_dec lo BASE.zero); destruct (BASE.eq_dec hi BASE.zero);
+    unfold zero in Hnz; subst; try contradiction; simpl;
+    try rewrite <- (BASE.non_zero_is_not_zero hi);
+    try rewrite <- (BASE.non_zero_is_not_zero lo);
+    try rewrite (BASE.non_zero_is_not_zero hi);
+    try rewrite (BASE.non_zero_is_not_zero lo);
+    try rewrite BASE.zero_is_zero; 
+    auto.
+  Qed.
 End DOUBLE.
 
 Module INT1 <: VALUE.
   Definition t := bit.
+
+  Definition is_zero v :=
+    match v with
+    | I => false
+    | O => true
+    end.
+
+  Definition zero: t := O.
+
+  Lemma eq_dec: forall (x: t) (y: t), {x = y} + {x <> y}.
+  Proof.
+    intros x y.
+    destruct x; destruct y; auto; right; intros contra; inversion contra.
+  Qed.
+
+  Lemma zero_is_zero: is_zero zero = true.
+  Proof. reflexivity. Qed.
+
+  Lemma non_zero_is_not_zero: forall (x: t), x <> zero -> is_zero x = false.
+  Proof. intros x Hnz; destruct x; [reflexivity|contradiction]. Qed.
 End INT1.
 
 Module INT2 := DOUBLE INT1.
@@ -43,28 +107,98 @@ Module INT32 := DOUBLE INT16.
 
 Module INT64 := DOUBLE INT32.
 
-
-
-Definition nibble := INT4.t.
-Definition byte := INT8.t.
-Definition word := INT16.t.
-Definition dword := INT32.t.
-
 Inductive sym : Type :=
+  (* Pointer to the program arguments. *)
+  | SInit (object: positive) (offset: positive)
+  (* Pointer into a stack frame *)
   | SFrame (frame: positive) (object: positive) (offset: positive)
+  (* Pointer to a global data item *)
   | SAtom (object: positive) (offset: positive)
-  | SAlloc (object: positive) (offset: positive)
+  (* Pointer to a function. *)
   | SFunc (func: name)
   .
 
-Inductive qword : Type :=
-  | QVal (val: INT64.t)
-  | QSym (val: sym)
+Inductive value : Type :=
+  | V8 (v: INT8.t)
+  | V16 (v: INT16.t)
+  | V32 (v: INT32.t)
+  | V64 (v: INT64.t)
+  | VSym (v: sym)
+  | VUnd
   .
 
-Inductive value : Type :=
-  | Val8 (v: INT8.t)
-  | Val16 (v: INT16.t)
-  | Val32 (v: INT32.t)
-  | Val64 (v: INT64.t)
+Inductive quad : Type :=
+  | QVal (v: INT64.t)
+  | QSym (v: sym)
+  | QUnd
   .
+
+Definition is_true (v: value): bool :=
+  match v with
+  | V8 v => negb (INT8.is_zero v)
+  | V16 v => negb (INT16.is_zero v)
+  | V32 v => negb (INT32.is_zero v)
+  | V64 v => negb (INT64.is_zero v)
+  | VSym _ => true
+  | VUnd => false
+  end.
+
+Inductive IsTrue: value -> Prop :=
+  | is_true_v8:  forall (v: INT8.t)  (NZ: v <> INT8.zero),  IsTrue (V8 v)
+  | is_true_v16: forall (v: INT16.t) (NZ: v <> INT16.zero), IsTrue (V16 v)
+  | is_true_v32: forall (v: INT32.t) (NZ: v <> INT32.zero), IsTrue (V32 v)
+  | is_true_v64: forall (v: INT64.t) (NZ: v <> INT64.zero), IsTrue (V64 v)
+  | is_true_sym: forall (s: sym), IsTrue (VSym s)
+  .
+
+Lemma is_true_True:
+  forall (v: value),
+    is_true v = true <-> IsTrue v.
+Proof.
+  intros v.
+  split; intros H.
+  {
+    destruct v; try constructor; inversion H as [H']; clear H;
+    intros contra; subst; simpl in H'; inversion H'.
+  }
+  {
+    inversion H; subst; clear H; auto; simpl;
+      [ rewrite INT8.non_zero_is_not_zero
+      | rewrite INT16.non_zero_is_not_zero
+      | rewrite INT32.non_zero_is_not_zero
+      | rewrite INT64.non_zero_is_not_zero
+      ]; auto.
+  }
+Qed.
+
+Inductive IsFalse: value -> Prop :=
+  | is_false_v8:  IsFalse (V8  INT8.zero)
+  | is_false_v16: IsFalse (V16 INT16.zero)
+  | is_false_v32: IsFalse (V32 INT32.zero)
+  | is_false_v64: IsFalse (V64 INT64.zero)
+  | is_false_und: IsFalse VUnd
+  .
+
+Lemma is_true_False:
+  forall (v: value),
+    is_true v = false <-> IsFalse v.
+Proof.
+  intros v.
+  split; intros H.
+  {
+    destruct v; try constructor; inversion H as [H'];
+      [ destruct (INT8.eq_dec v INT8.zero)
+      | destruct (INT16.eq_dec v INT16.zero)
+      | destruct (INT32.eq_dec v INT32.zero)
+      | destruct (INT64.eq_dec v INT64.zero)
+      ]; subst; try constructor;
+      [ rewrite INT8.non_zero_is_not_zero in H'
+      | rewrite INT16.non_zero_is_not_zero in H'
+      | rewrite INT32.non_zero_is_not_zero in H'
+      | rewrite INT64.non_zero_is_not_zero in H'
+      ]; auto; inversion H'.
+  }
+  {
+    inversion H; subst; simpl; reflexivity.
+  }
+Qed.
